key util lemmas

steel/Zeta.Steel.KeyUtils.fst
@@ -45,22 +45,110 @@ let is_proper_descendent_key_type (k0 k1:T.internal_key)
     [SMTPat (is_proper_descendent k0 k1)]
   = ()
 
+let bit_offset_in_word (i:U16.t { U16.v i < 256 })
+  : U32.t & U32.t
+  = let open U16 in
+    if i <^ 64us
+    then 0ul, C.uint16_to_uint32 i
+    else if i <^ 128us
+    then 1ul, C.uint16_to_uint32 (i -^ 64us)
+    else if i <^ 192us
+    then 2ul, C.uint16_to_uint32 (i -^ 128us)
+    else 3ul, C.uint16_to_uint32 (i -^ 192us)
+
+let nth_63_mod2 (x:U64.t)
+  : Lemma (UInt.nth (U64.v x) 63 == (U64.v x % 2 = 1))
+  = ()
+
+let ith_bit_64 (x:U64.t) (i:U32.t { U32.v i < 64 })
+  : bool
+  = U64.shift_right x i `U64.rem` 2uL = 1uL
+
+let ith_bit_64_nth (x:U64.t) (i:U32.t { U32.v i < 64 })
+  : Lemma (ith_bit_64 x i == FStar.UInt.nth (U64.v x) (63 - U32.v i))
+  = calc (==) {
+      FStar.UInt.nth (U64.v (U64.shift_right x i)) 63;
+    (==) { FStar.UInt.shift_right_lemma_2 #64 (U64.v x) (U32.v i) 63 }
+      UInt.nth #64 (U64.v x) (63 - U32.v i);
+    }
+
 let ith_bit (k0:T.base_key) (i:U16.t { U16.v i < 256 })
   : bool
   = let open U16 in
     let kk = k0.T.k in
-    if i <^ 64us
-    then (U64.shift_right kk.T.v0 (C.uint16_to_uint32 i)) `U64.rem` 2uL = 1uL
-    else if i <^ 128us
-    then (U64.shift_right kk.T.v1 (C.uint16_to_uint32 (i -^ 64us))) `U64.rem` 2uL = 1uL
-    else if i <^ 192us
-    then (U64.shift_right kk.T.v2 (C.uint16_to_uint32 (i -^ 128us))) `U64.rem` 2uL = 1uL
-    else (U64.shift_right kk.T.v3 (C.uint16_to_uint32 (i -^ 192us))) `U64.rem` 2uL = 1uL
+    let word, bit = bit_offset_in_word i in
+    if word = 0ul
+    then ith_bit_64 kk.T.v0 bit
+    else if word = 1ul
+    then ith_bit_64 kk.T.v1 bit
+    else if word = 2ul
+    then ith_bit_64 kk.T.v2 bit
+    else ith_bit_64 kk.T.v3 bit
 
-assume
-val lift_base_key (k: T.base_key)
-  : GTot (k':Zeta.Key.base_key { Zeta.BinTree.depth k' = U16.v k.significant_digits })
+let set_ith_bit (k0:T.base_key) (i:U16.t { U16.v i < 256 })
+  : GTot T.base_key
+  = let open U16 in
+    let kk = k0.T.k in
+    let word, bit = bit_offset_in_word i in
+    let mask = U64.shift_left 1uL bit in
+    let kk' =
+      if word = 0ul
+      then { kk with v0 = kk.v0 `U64.logor` mask  }
+      else if word = 1ul
+      then { kk with v1 = kk.v1 `U64.logor` mask }
+      else if word = 2ul
+      then { kk with v2 = kk.v2 `U64.logor` mask }
+      else { kk with v3 = kk.v3 `U64.logor` mask }
+    in
+    { k0 with k = kk' }
 
+#push-options "--fuel 0 --ifuel 0"
+let set_get_ith_bit_core (k:T.base_key) (i:U16.t { U16.v i < 256 })
+  : Lemma ((ith_bit (set_ith_bit k i) i == true))
+  = let open U16 in
+    let k' = set_ith_bit k i in
+    let word, index = bit_offset_in_word i in
+    let kk =
+      if word = 0ul then k'.k.v0
+      else if word = 1ul then k'.k.v1
+      else if word = 2ul then k'.k.v2
+      else k'.k.v3
+    in
+    let res = ith_bit_64 kk index in
+    let mask = U64.shift_left 1uL index in
+      calc (==) {
+        ith_bit k' i;
+       (==) { }
+        ith_bit_64 kk index;
+       (==) { ith_bit_64_nth kk index }
+        UInt.nth #64 (U64.v kk) (63 - U32.v index);
+       (==) {}
+        UInt.nth #64 (U64.v (kk `U64.logor` mask)) (63 - U32.v index);
+       (==) { UInt.logor_definition #64 (U64.v kk) (U64.v mask) (63 - U32.v index) }
+        (UInt.nth #64 (U64.v kk) (63 - U32.v index) ||
+         UInt.nth #64 (U64.v mask) (63 - U32.v index));
+       (==) { UInt.shift_left_lemma_2 #64 1 (U32.v index) (63 - U32.v index) }
+        (UInt.nth #64 (U64.v kk) (63 - U32.v index) ||
+         UInt.nth #64 1 63);
+       (==) { nth_63_mod2 1uL }
+       (UInt.nth #64 (U64.v kk) (63 - U32.v index) ||
+        (1%2 = 1));
+       (==) {}
+        true;
+      }
+#pop-options
+
+let set_ith_bit_modifies (k:T.base_key)
+                         (i:U16.t { U16.v i < 256 })
+                         (j:U16.t { U16.v j <> U16.v i /\ U16.v j < 256 })
+  : Lemma ((ith_bit (set_ith_bit k i) j == ith_bit k j))
+  = admit()
+
+let set_get_ith_bit (k:T.base_key) (i:U16.t { U16.v i < 256 })
+  : Lemma ((ith_bit (set_ith_bit k i) i == true) /\
+            (forall (j:U16.t { j <> i /\ U16.v j < 256 }). ith_bit (set_ith_bit k i) j == ith_bit k j))
+  = set_get_ith_bit_core k i;
+    FStar.Classical.forall_intro (set_ith_bit_modifies k i)
 
 let root_base_key: T.base_key =
   let open T in
@@ -71,23 +159,17 @@ let root_base_key: T.base_key =
 
 let root_key: T.key = InternalKey root_base_key
 
+let ith_bit_root_base_key (i:U16.t { U16.v i < 256 })
+  : Lemma (ith_bit root_base_key i == false)
+  = let open U16 in
+    let res = ith_bit root_base_key i in
+    let kk = root_base_key.k in
+    let word, bit = bit_offset_in_word i in
+    FStar.UInt.shift_right_value_lemma #64 0 (U32.v bit);
+    FStar.Math.Lemmas.small_div 0 (pow2 (U32.v bit))
+
 (* if you lift a lowered key, you get the original key, but not the other way round *)
-#push-options "--query_stats"
-assume
-val shift_left_256 (i:u256) (n:U16.t { U16.v n < 256 })
-  : u256
-let shift_left_key (k:T.base_key { U16.v k.significant_digits < 256 })
-  : T.base_key
-  = let key = shift_left_256 k.k 1us in
-    { k with k=key; significant_digits = U16.(k.significant_digits +^ 1us) }
-
-assume
-val shift_left_256_lemma (k:T.base_key { U16.v k.significant_digits < 256 })
-  : Lemma ((forall (i:U16.t { U16.v i < 255 }).
-              ith_bit k i == ith_bit (shift_left_key k) U16.(i +^ 1us)) /\
-            ith_bit (shift_left_key k) 0us = false)
-
-let rec lift_base_key' (k: T.base_key)
+let rec lift_base_key (k: T.base_key)
   : GTot (k':Zeta.Key.base_key {
                Zeta.BinTree.depth k' = U16.v k.significant_digits
           })
@@ -96,45 +178,74 @@ let rec lift_base_key' (k: T.base_key)
     let open Zeta.BinTree in
     if k.significant_digits = 0us then Root
     else let i = k.significant_digits -^ 1us in
-         let k' = lift_base_key' ({k with significant_digits = i }) in
+         let k' = lift_base_key ({k with significant_digits = i }) in
          if ith_bit k i
          then RightChild k'
          else LeftChild k'
 
 let rec lower_base_key' (k: Zeta.Key.base_key)
   : GTot (k':T.base_key {
-       //        lift_base_key k' = k /\
                 U16.v k'.significant_digits = Zeta.BinTree.depth k
           })
   = let open Zeta.BinTree in
     match k with
     | Root -> root_base_key
-    | LeftChild k -> shift_left_key (lower_base_key' k)
-    | RightChild k ->
-      let k = shift_left_key (lower_base_key' k) in
-      let key = {k.k with v0 = k.k.v0 `U64.logxor` 1uL} in
-      {k with k = key }
 
+    | LeftChild k ->
+      let k' = lower_base_key' k in
+      { k' with significant_digits = U16.(k'.significant_digits +^ 1us) }
+
+    | RightChild k ->
+      let k' = lower_base_key' k in
+      let k'' = { k' with significant_digits = U16.(k'.significant_digits +^ 1us) } in
+      set_ith_bit k'' k'.significant_digits
+
+
+let rec lower_base_key_significant_digits (k: Zeta.Key.base_key)
+  : Lemma (let k' = lower_base_key' k in
+           U16.v k'.significant_digits = Zeta.BinTree.depth k /\
+           (forall (i:U16.t). Zeta.BinTree.depth k <= U16.v i /\
+                         U16.v i < 256 ==>
+                         ith_bit k' i == false))
+  = let open Zeta.BinTree in
+    match k with
+    | Root ->
+      FStar.Classical.forall_intro ith_bit_root_base_key
+
+    | LeftChild k ->
+      lower_base_key_significant_digits k
+
+    | RightChild k ->
+      lower_base_key_significant_digits k;
+      let kk = lower_base_key' k in
+      set_get_ith_bit kk kk.significant_digits
+
+#push-options "--query_stats --fuel 2 --ifuel 1 --z3rlimit_factor 4"
 let rec lift_lower_id (k:Zeta.Key.base_key)
-  : Lemma (lift_base_key' (lower_base_key' k) == k)
+  : Lemma (lift_base_key (lower_base_key' k) == k)
   = let open U16 in
     let open Zeta.BinTree in
     match k with
     | Root -> ()
     | LeftChild k ->
       lift_lower_id k;
+      lower_base_key_significant_digits k
+    | RightChild k ->
+      lift_lower_id k;
       let k0 = lower_base_key' k in
-      let i = k0.significant_digits in
-      shift_left_256_lemma k0;
-      assume (ith_bit k0 i = false);
-      admit()
-    | _ -> admit()
+      assert (lift_base_key k0 == k);
+      let res = {set_ith_bit k0 k0.significant_digits with significant_digits = U16.(k0.significant_digits +^ 1us) } in
+      set_get_ith_bit k0 k0.significant_digits;
+      assert (lower_base_key' (RightChild k) == res)
 
-assume
-val lower_base_key (k: Zeta.Key.base_key)
+
+
+let lower_base_key (k: Zeta.Key.base_key)
   : GTot (k':T.base_key {
                 lift_base_key k' = k
           })
+  = lift_lower_id k;
+    lower_base_key' k
 
 let desc_dir (k0:T.base_key) (k1:T.base_key { k0 `is_proper_descendent` k1 })
   : bool
